compiler/backend/semantics/patSemScript.sml
@@ -147,9 +147,6 @@ val _ = Datatype`
      ; compile_oracle : num -> 'c # patLang$exp list
      |>`;
 
-
-(*  v store and v store_v list are same types *)
-
 (* get_carg_pat “v store  -> c_type -> v -> c_value option” *)
 val get_carg_pat_def = Define `
    (get_carg_pat (_:patSem$v store) (C_array conf) (Litv(StrLit s)) =
@@ -174,15 +171,6 @@ val get_carg_pat_def = Define `
 /\ (get_carg_pat _ _ _ = NONE)`
 
 
-(*
-val get_cargs_pat_def = Define
-  `(get_cargs_pat s [] [] = SOME [])
-/\ (get_cargs_pat s (ty::tys) (arg::args) =
-    OPTION_MAP2 CONS (get_carg_pat s ty arg) (get_cargs_pat s tys args))
-/\ (get_cargs_pat _ _ _ = NONE)
-`
-*)
-
 val ret_val_pat_def = Define
 `(ret_val_pat (SOME(C_boolv b)) = Boolv b)
 /\ (ret_val_pat (SOME(C_intv i)) = Litv(IntLit i))
@@ -193,69 +181,6 @@ val store_carg_pat_def = Define `
    (store_carg_pat (s:patSem$v store) (Loc lnum) ws =
     store_assign lnum (W8array ws) s)
 /\ (store_carg_pat s _ _ = SOME s)`
-
-(*
-val store_cargs_pat_def = Define
-  `(store_cargs_pat [] [] s = SOME s)
-/\ (store_cargs_pat (marg::margs) (w::ws) s =
-      case store_carg_pat s marg w of
-        | SOME s' => store_cargs_pat margs ws s'
-        | NONE => NONE)
-/\ (store_cargs_pat _ _ s = SOME s)
-`
-
-
-val do_ffi_pat_def = Define `
-  do_ffi_pat (t:('ffi, 'c) patSem$state) n args =
-   case FIND (\x.x.mlname = n) (debug_sig::t.ffi.signatures) of SOME sign =>
-     (case get_cargs_pat t.refs sign.args args of
-          SOME cargs =>
-           (case call_FFI t.ffi n sign cargs (als_args sign.args args) of
-              SOME (FFI_return t' newargs retv) =>
-                (case store_cargs_pat (get_mut_args sign.args args) newargs (t.refs) of
-                  | SOME s' => SOME (t with <| refs := s'; ffi := t'|>, Rval (ret_val_pat retv))
-                  | NONE => NONE)
-            | SOME (FFI_final outcome) => SOME (t, Rerr (Rabort (Rffi_error outcome)))
-            | NONE => NONE)
-        | NONE => NONE)
-   | NONE => NONE
-  `
-(* defs for abstract ffi  *)
-
-val do_ffi_wrp_def = Define `
-  do_ffi_wrp st name args =
-   case ffi$do_ffi st ((\s. s.ffi) st) (st.refs) store_carg_pat (get_carg_pat st.refs) name args of
-     | NONE => NONE
-     | SOME (INL outcome) => SOME (st, Rerr (Rabort (Rffi_error outcome)))
-     | SOME (INR (ffi', s', retv)) =>
-         SOME (st with <| refs := s'; ffi := ffi'|>, Rval (ret_val_pat retv))`
-
-Theorem get_cargs_pat_get_cargs_eq:
-  !st cts args l. get_cargs_pat st cts args = l ==>
-     get_cargs (get_carg_pat st) cts args = l
-Proof
-  ho_match_mp_tac (fetch "-" "get_cargs_pat_ind") >>
-  rw [ffiTheory.get_cargs_def, (fetch "-" "get_cargs_pat_def")]
-QED
-
-
-Theorem store_cargs_pat_store_cargs_eq:
-  !ms ws s s'. store_cargs_pat ms ws s = s' ==>
-     store_cargs s store_carg_pat ms ws = s'
-Proof
-  ho_match_mp_tac (fetch "-" "store_cargs_pat_ind") >>
-  rw [ffiTheory.store_cargs_def, (fetch "-" "store_cargs_pat_def")] >>
-  cases_on `marg` >> fs [(fetch "-" "store_carg_pat_def")] >> every_case_tac >> fs []
-QED
-
-Theorem do_ffi_pat_do_ffi_wrp_eq:
-  do_ffi_pat st n args =  do_ffi_wrp st n args
-Proof
-  rw [do_ffi_pat_def, do_ffi_wrp_def, ffiTheory.do_ffi_def] >>
-  every_case_tac >> imp_res_tac get_cargs_pat_get_cargs_eq >>
-  imp_res_tac store_cargs_pat_store_cargs_eq >> fs [] >> rveq >> rfs []
-QED
-*)
 
 val do_app_def = Define `
  (do_app s (op : patLang$op) vs =
